EvenOddProgram.thy
@@ -1,0 +1,372 @@
+theory EvenOddProgram
+  imports "HOL-Library.AList_Mapping" "VCG"
+begin
+
+section "Even/odd Functions"
+
+definition odd_entry :: "llvm_instruction_block" where
+  "odd_entry \<equiv> (
+    [],
+    [
+      alloca (%''n.addr'') i32 (Some 4),
+      store i32 (reg %''n'') (reg %''n.addr'') (Some 4),
+      load (%''0'') i32 (reg %''n.addr'') (Some 4),
+      call (Some %''call'') i1 (@''even'') [(i32, reg %''0'')],
+      icmp (%''lnot'') False comp_eq i1 (reg %''call'') (val (vi1 False))
+    ],
+    ret (Some (i1, (reg %''lnot'')))
+  )"
+
+definition odd_func :: "llvm_function" where
+  "odd_func \<equiv> func i1 [(%''n'', i32)]
+    [
+      (%''entry'', odd_entry)
+    ]"
+
+
+definition even_entry :: "llvm_instruction_block" where
+  "even_entry \<equiv> (
+    [],
+    [
+      alloca (%''retval'') i1 (Some 1),
+      alloca (%''n.addr'') i32 (Some 4),
+      store i32 (reg %''n'') (reg %''n.addr'') (Some 4),
+      load (%''0'') i32 (reg %''n.addr'') (Some 4),
+      icmp (%''cmp'') False comp_eq i32 (reg %''0'') (val (vi32 0))
+    ],
+    br_i1 (reg %''cmp'') (%''if.then'') (%''if.else'')
+  )"
+definition even_if :: "llvm_instruction_block" where
+  "even_if \<equiv> (
+    [],
+    [
+      store i1 (val (vi1 True)) (reg %''retval'') (Some 1)
+    ],
+    br_label (%''return'')
+  )"
+definition even_else :: "llvm_instruction_block" where
+  "even_else \<equiv> (
+    [],
+    [
+      load (%''1'') i32 (reg %''n.addr'') (Some 4),
+      add (%''sub'') add_nsw i32 (reg %''1'') (val (vi32 (-1))),
+      call (Some %''call'') i1 (@''odd'') [(i32, reg %''sub'')],
+      store i1 (reg %''call'') (reg %''retval'') (Some 1)
+    ],
+    br_label (%''return'')
+  )"
+definition even_return :: "llvm_instruction_block" where
+  "even_return \<equiv> (
+    [],
+    [
+      load (%''2'') i32 (reg %''retval'') (Some 4)
+    ],
+    ret (Some (i1, (reg %''2'')))
+  )"
+
+definition even_func :: "llvm_function" where
+  "even_func \<equiv> func i1 [(%''n'', i32)]
+    [
+      (%''entry'', even_entry),
+      (%''if.then'', even_if),
+      (%''if.else'', even_else),
+      (%''return'', even_return)
+    ]"
+
+abbreviation even_annots :: "precondition * block_preconditions * postcondition" where
+  "even_annots \<equiv> (
+    (\<lambda>s.
+      \<exists>n. register_\<alpha> s (reg %''n'') = Some (vi32 n)
+    \<and> 0 \<le>s n
+    ),
+    [],
+    (\<lambda>s s' v.
+      \<exists>n b a1 a2. register_\<alpha> s (reg %''n'') = Some (vi32 n)
+    \<and> v = Some (vi1 (even n))
+    \<and> memory_\<alpha> s' = (memory_\<alpha> s)(saddr a1 := Some (mem_val (vi32 n)), saddr a2 := Some (mem_val (vi1 b)))
+    \<and> memory_\<alpha> s (saddr a1) = None
+    \<and> memory_\<alpha> s (saddr a2) = None
+    \<and> (\<forall>n. register_\<alpha> s' (reg @n) = register_\<alpha> s (reg @n))
+    )
+  )"
+abbreviation odd_annots :: "precondition * block_preconditions * postcondition" where
+  "odd_annots \<equiv> (
+    (\<lambda>s.
+      \<exists>n. register_\<alpha> s (reg %''n'') = Some (vi32 n)
+    \<and> 0 \<le>s n
+    ),
+    [],
+    (\<lambda>s s' v.
+      \<exists>n ad. register_\<alpha> s (reg %''n'') = Some (vi32 n)
+    \<and> v = Some (vi1 (odd n))
+    \<and> memory_\<alpha> s' = (memory_\<alpha> s)(saddr ad := Some (mem_val (vi32 n)))
+    \<and> memory_\<alpha> s (saddr ad) = None
+    \<and> (\<forall>n. register_\<alpha> s' (reg @n) = register_\<alpha> s (reg @n))
+    )
+  )"
+
+definition even_odd_prog :: "llvm_program" where
+  "even_odd_prog \<equiv> [
+    (@''even'', even_func),
+    (@''odd'',  odd_func)
+  ]"
+
+definition even_odd_annots :: "annotations" where
+  "even_odd_annots \<equiv> [
+    (@''even'', even_annots),
+    (@''odd'',  odd_annots)
+  ]"
+
+lemma register_\<alpha>_pop_contract [simp]:
+  "register_\<alpha> (pop_frame s s') ref = (
+     case ref of
+       reg (lid n) \<Rightarrow> register_\<alpha> s (reg (lid n))
+     | reg (gid n) \<Rightarrow> register_\<alpha> s' (reg (gid n))
+     | val v       \<Rightarrow> Some v)"
+  by (cases s; cases s'; cases ref; auto split: llvm_value_ref.splits llvm_identifier.splits) 
+fun stack_len :: "state \<Rightarrow> nat" where
+  "stack_len (lr, gr, sm, hm, gm) = length sm"
+
+lemma memory_\<alpha>_pop_saddr [simp]:
+  "memory_\<alpha> (pop_frame s s') (saddr a) = 
+     (if memory_\<alpha> s (saddr a) \<noteq> None then memory_\<alpha> s' (saddr a) else None)"
+  by (cases s; cases s'; simp add: single_memory_\<alpha>_def allocated_single_memory_address_def)
+
+lemma memory_\<alpha>_pop_haddr [simp]:
+  "memory_\<alpha> (pop_frame s s') (haddr a) = memory_\<alpha> s' (haddr a)"
+  by (cases s; cases s'; simp)
+
+lemma memory_\<alpha>_pop_gaddr [simp]:
+  "memory_\<alpha> (pop_frame s s') (gaddr a) = memory_\<alpha> s' (gaddr a)"
+  by (cases s; cases s'; simp)
+
+
+lemma register_\<alpha>_push_frame [simp]:
+  "register_\<alpha> (push_frame s) (reg (lid n)) = None"
+  "register_\<alpha> (push_frame s) (reg (gid n)) = register_\<alpha> s (reg (gid n))"
+  by (cases s; simp)+
+
+lemma memory_\<alpha>_push_frame [simp]:
+  "memory_\<alpha> (push_frame s) = memory_\<alpha> s"
+  apply (rule ext) subgoal for ad
+    by (cases s; cases ad; simp)
+  done
+
+
+
+
+
+lemma contract_updates_register[simp]:
+  assumes trace_link: "\<And>r. register_\<alpha> callee_state (reg @r) = f (reg @r)"
+  assumes frame_invariant: "\<And>r name. r = reg @name \<Longrightarrow> f r = register_\<alpha> caller_state r"
+  shows "register_\<alpha> (pop_frame caller_state callee_state) = register_\<alpha> caller_state"
+  apply (rule ext)
+  subgoal for n apply (cases n)
+  subgoal for name apply (cases name)
+    using assms by (auto )
+  by simp done
+
+lemma pop_frame_peel_gaddr [simp]:
+  "(\<lambda>a. case a of saddr sa \<Rightarrow> if M a \<noteq> None then (C (gaddr ga \<mapsto> v)) a else None | _ \<Rightarrow> (C (gaddr ga \<mapsto> v)) a) =
+   ((\<lambda>a. case a of saddr sa \<Rightarrow> if M a \<noteq> None then C a else None | _ \<Rightarrow> C a) (gaddr ga \<mapsto> v))"
+  apply (rule ext) subgoal for a by (cases a) auto done
+
+lemma pop_frame_peel_haddr [simp]:
+  "(\<lambda>a. case a of saddr sa \<Rightarrow> if M a \<noteq> None then (C (haddr ha \<mapsto> v)) a else None | _ \<Rightarrow> (C (haddr ha \<mapsto> v)) a) =
+   ((\<lambda>a. case a of saddr sa \<Rightarrow> if M a \<noteq> None then C a else None | _ \<Rightarrow> C a) (haddr ha \<mapsto> v))"
+  apply (rule ext) subgoal for a by (cases a) auto done
+
+lemma pop_frame_peel_saddr [simp]:
+  "(\<lambda>a. case a of saddr sa' \<Rightarrow> if M a \<noteq> None then (C (saddr sa \<mapsto> v)) a else None | _ \<Rightarrow> (C (saddr sa \<mapsto> v)) a) =
+   (if M (saddr sa) \<noteq> None 
+    then ((\<lambda>a. case a of saddr sa' \<Rightarrow> if M a \<noteq> None then C a else None | _ \<Rightarrow> C a) (saddr sa \<mapsto> v))
+    else (\<lambda>a. case a of saddr sa' \<Rightarrow> if M a \<noteq> None then C a else None | _ \<Rightarrow> C a))"
+  apply (rule ext) subgoal for a by (cases a) auto done
+
+lemma pop_frame_M_drop_saddr [simp]:
+  "C (saddr sa') = None \<Longrightarrow>
+   (\<lambda>a. case a of saddr sa \<Rightarrow> if (M(saddr sa' \<mapsto> v)) a \<noteq> None then C a else None | _ \<Rightarrow> C a) =
+   (\<lambda>a. case a of saddr sa \<Rightarrow> if M a \<noteq> None then C a else None | _ \<Rightarrow> C a)"
+  apply (rule ext) subgoal for a by (cases a) auto done
+
+lemma pop_frame_peel_absolute_base [simp]:
+  "(\<lambda>a. case a of saddr sa \<Rightarrow> if C a \<noteq> None then C a else None | _ \<Rightarrow> C a) = C"
+  apply (rule ext) subgoal for a by (cases a) auto done
+
+lemma memory_pop_frame [simp]:
+  assumes "memory_\<alpha> x = X"
+  assumes "memory_\<alpha> y = Y"
+  shows "memory_\<alpha> (pop_frame x y) = (\<lambda>a. case a of saddr sa \<Rightarrow> if X a \<noteq> None then Y a else None | _ \<Rightarrow> Y a)"
+  apply (rule ext) subgoal for a using assms by (cases a) auto done
+
+
+lemma verify_even_odd:
+  "verify_program even_odd_prog even_odd_annots"
+  apply (vcg_verify_program prog: even_odd_prog_def annot: even_odd_annots_def)
+  apply (unfold_first_label func: even_func_def)
+    apply (unfold_first_label func: even_func_def)
+    apply (intro allI impI)
+  subgoal for s
+    apply (vcg_floyd_cond prog: even_odd_prog_def func: even_func_def)
+    apply clean_assms
+    apply (vcg_steps_execi block: even_entry_def)
+    apply vcg_steps_execi
+    apply vcg_steps_execi
+    apply vcg_steps_execi
+    apply vcg_steps_execi
+    apply vcg_steps_execi
+    subgoal for n rva na s'
+      apply (vcg_steps_flowi_branch prog: even_odd_prog_def annot: even_odd_annots_def)
+      apply (vcg_step prog: even_odd_prog_def func: even_func_def)
+      apply (vcg_steps_execi block: even_if_def)
+      apply vcg_steps_execi
+      apply (vcg_steps_flowi_branch prog: even_odd_prog_def annot: even_odd_annots_def)
+      apply (vcg_step prog: even_odd_prog_def func: even_func_def)
+      apply (vcg_steps_execi block: even_return_def)
+      apply vcg_steps_execi
+      apply (vcg_steps_flowi_return prog: even_odd_prog_def annot: even_odd_annots_def)
+      apply (vcg_annotation_holds prog: even_odd_prog_def annot: even_odd_annots_def pre: even_odd_annots_def)
+      unfolding even_odd_prog_def
+      by (auto split: if_splits)
+    subgoal for n rva na s'
+      apply (vcg_steps_flowi_branch prog: even_odd_prog_def annot: even_odd_annots_def)
+      apply (vcg_step prog: even_odd_prog_def func: even_func_def)
+      apply (vcg_steps_execi block: even_else_def)
+      apply (vcg_steps_execi)
+      apply (vcg_steps_execi)
+         apply (subst even_odd_prog_def)
+         apply simp
+        apply (unfold_first_label func: odd_func_def)
+       apply (subst even_odd_annots_def)
+       apply simp
+      apply (simp only: prepare_state.simps)
+      apply (subst odd_func_def)
+      apply (simp (no_asm) del: assign_params.simps split_paired_All)
+      apply (intro wp_assign_params_intro wp_assign_params_empty_intro) apply simp apply simp
+      apply (intro conjI)
+      apply (smt (verit, del_insts) add.inverse_neutral add_diff_cancel_right' diff_minus_eq_add fun_upd_same signed.nle_le signed_arith_eq_checks_to_ord(1) signed_minus_1
+          word_sle_eq)
+      apply (intro allI impI)
+      apply (elim exE conjE)
+      apply (rule wp_restore_state_intro)
+        apply blast defer
+       apply blast
+      apply (intro wp_intro)
+        apply fastforce defer
+       apply blast
+        apply (elim conjE)
+  apply simp
+  apply (hypsubst_thin)+
+  apply (subst (asm) fun_upd_apply[symmetric])+
+  apply clean_assms
+      apply vcg_steps_execi
+      apply vcg_steps_execi
+      apply (vcg_steps_flowi_branch prog: even_odd_prog_def annot: even_odd_annots_def)
+      apply (vcg_step prog: even_odd_prog_def func: even_func_def)
+      apply (vcg_steps_execi block: even_return_def)
+
+      apply vcg_steps_execi
+      apply (vcg_steps_flowi_return prog: even_odd_prog_def annot: even_odd_annots_def)
+      apply (vcg_annotation_holds prog: even_odd_prog_def annot: even_odd_annots_def pre: even_odd_annots_def)
+      unfolding even_odd_prog_def apply (intro conjI) apply simp apply blast apply (auto split: if_splits)
+      by fast
+    done
+  apply (unfold_first_label func: odd_func_def)
+  apply (unfold_first_label func: odd_func_def)
+  apply (intro allI impI)
+  subgoal for s
+    apply (vcg_floyd_cond prog: even_odd_prog_def func: odd_func_def)
+    apply clean_assms
+    apply (vcg_steps_execi block: odd_entry_def)
+    apply vcg_steps_execi
+    apply vcg_steps_execi
+    apply vcg_steps_execi
+         apply (subst even_odd_prog_def)
+         apply simp
+        apply (unfold_first_label func: even_func_def)
+       apply (subst even_odd_annots_def)
+       apply simp
+      apply (simp only: prepare_state.simps)
+      apply (subst even_func_def)
+      apply (simp (no_asm) del: assign_params.simps split_paired_All)
+      apply (intro wp_assign_params_intro wp_assign_params_empty_intro) apply simp apply simp
+    apply (intro conjI)
+     apply simp
+      apply (intro allI impI)
+      apply (elim exE conjE)
+      apply (rule wp_restore_state_intro)
+        apply blast defer
+       apply blast
+      apply (intro wp_intro)
+        apply fastforce defer
+       apply blast
+        apply (elim conjE)
+  apply simp
+  apply (hypsubst_thin)+
+  apply (subst (asm) fun_upd_apply[symmetric])+
+  apply clean_assms
+  apply vcg_steps_execi
+  apply vcg_steps_execi
+      apply (vcg_steps_flowi_return prog: even_odd_prog_def annot: even_odd_annots_def)
+      apply (vcg_annotation_holds prog: even_odd_prog_def annot: even_odd_annots_def pre: even_odd_annots_def)
+      unfolding even_odd_prog_def by (auto split: if_splits)
+    done  
+
+
+(*
+define dso_local noundef zeroext i1 @odd(int)(i32 noundef %n) {
+entry:
+  %n.addr = alloca i32, align 4
+  store i32 %n, ptr %n.addr, align 4
+  %0 = load i32, ptr %n.addr, align 4
+  %sub = sub nsw i32 %0, 1
+  %call = call noundef zeroext i1 @even(int)(i32 noundef %sub)
+  %lnot = xor i1 %call, true
+  ret i1 %lnot
+}
+
+define dso_local noundef zeroext i1 @even(int)(i32 noundef %n) {
+entry:
+  %retval = alloca i1, align 1
+  %n.addr = alloca i32, align 4
+  store i32 %n, ptr %n.addr, align 4
+  %0 = load i32, ptr %n.addr, align 4
+  %cmp = icmp eq i32 %0, 0
+  br i1 %cmp, label %if.then, label %if.else
+
+if.then:
+  store i1 true, ptr %retval, align 1
+  br label %return
+
+if.else:
+  %1 = load i32, ptr %n.addr, align 4
+  %call = call noundef zeroext i1 @odd(int)(i32 noundef %1)
+  %lnot = xor i1 %call, true
+  store i1 %lnot, ptr %retval, align 1
+  br label %return
+
+return:
+  %2 = load i1, ptr %retval, align 1
+  ret i1 %2
+}
+
+
+*)
+
+
+
+
+
+
+
+
+
+
+
+
+
+
+
+
+
+end
