MultProgram.thy
@@ -1,0 +1,376 @@
+theory MultProgram
+  imports "HOL-Library.AList_Mapping" "VCG"
+begin
+
+
+section "Mult Function"
+
+definition mult_entry :: "llvm_instruction_block" where
+  "mult_entry = (
+    [],
+    [
+      alloca (lid ''a.addr'') i32 (Some 4),
+      alloca (lid ''b.addr'') i32 (Some 4),
+      alloca (lid ''result'') i32 (Some 4),
+      alloca (lid ''i'') i32 (Some 4),
+      store i32 (reg (lid ''a'')) (reg (lid ''a.addr'')) (Some 4),
+      store i32 (reg (lid ''b'')) (reg (lid ''b.addr'')) (Some 4),
+      store i32 (val (vi32 0)) (reg (lid ''result'')) (Some 4),
+      store i32 (val (vi32 0)) (reg (lid ''i'')) (Some 4)
+    ],
+    br_label (lid ''for.cond'')
+  )"
+
+
+definition mult_pre :: "precondition" where
+  "mult_pre = (\<lambda>s. \<exists>a b.
+    register_contains_value (lid ''a'') (vi32 a) s
+  \<and> register_contains_value (lid ''b'') (vi32 b) s
+  \<and> - (2 ^ 31) \<le> sint a * sint b
+  \<and> sint a * sint b \<le> 2 ^ 31 - 1
+  \<and> 0 <s b
+  \<and> b \<le>s 2 ^ 31 - 1
+  )"
+
+(*
+2 entry:
+3 %a.addr = alloca i32, align 4
+4 %b.addr = alloca i32, align 4
+5 %result = alloca i32, align 4
+6 %i = alloca i32, align 4
+7 store i32 %a, ptr %a.addr, align 4
+8 store i32 %b, ptr %b.addr, align 4
+9 store i32 0, ptr %result, align 4
+10 store i32 0, ptr %i, align 4
+11 br label %for.cond
+*)
+
+
+definition mult_cond :: "llvm_instruction_block" where
+  "mult_cond = (
+    [],
+    [
+      load (lid ''0'') i32 (reg (lid ''i'')) (Some 4),
+      load (lid ''1'') i32 (reg (lid ''b.addr'')) (Some 4),
+      icmp (lid ''cmp'') False comp_slt i32 (reg (lid ''0'')) (reg (lid ''1''))
+    ],
+    br_i1 (reg (lid ''cmp'')) (lid ''for.body'') (lid ''for.end'')
+  )"
+
+(*
+13 for.cond:
+14 %0 = load i32, ptr %i, align 4
+15 %1 = load i32, ptr %b.addr, align 4
+16 %cmp = icmp slt i32 %0, %1
+17 br i1 %cmp, label %for.body, label %for.end
+*)
+
+
+definition mult_body :: "llvm_instruction_block" where
+  "mult_body = (
+    [],
+    [
+      load (lid ''2'') i32 (reg (lid ''a.addr'')) (Some 4),
+      load (lid ''3'') i32 (reg (lid ''result'')) (Some 4),
+      add (lid ''add'') add_nsw i32 (reg (lid ''3'')) (reg (lid ''2'')),
+      store i32 (reg (lid ''add'')) (reg (lid ''result'')) (Some 4)
+    ],
+    br_label (lid ''for.inc'')
+  )"
+
+definition mult_body_pre :: "state \<Rightarrow> state \<Rightarrow> bool" where
+  "mult_body_pre = (\<lambda>s s'. \<exists>aa a ba b ia i resa.
+    register_contains_value ((%''a.addr'')) (addr aa) s'
+  \<and> register_contains_value ((%''i''))      (addr ia) s'
+  \<and> register_contains_value ((%''b.addr'')) (addr ba) s'
+  \<and> register_contains_value ((%''result'')) (addr resa) s'
+
+  \<and> register_contains_value ((%''a'')) (vi32 a) s
+  \<and> register_contains_value ((%''b'')) (vi32 b) s
+  \<and> register_contains_value ((%''a'')) (vi32 a) s'
+  \<and> register_contains_value ((%''b'')) (vi32 b) s'
+
+  \<and> memory_\<alpha> s' = (memory_\<alpha> s)(
+      aa   := Some (mem_val (vi32 a)),
+      ba   := Some (mem_val (vi32 b)),
+      ia   := Some (mem_val (vi32 i)),
+      resa := Some (mem_val (vi32 (a*i)))
+    )
+  \<and> unique_addresses [aa, ba, ia, resa]
+  \<and> 0 \<le>s i
+  \<and> i <s b
+  )"
+
+(*
+19 for.body:
+20 %2 = load i32, ptr %a.addr, align 4
+21 %3 = load i32, ptr %result, align 4
+22 %add = add nsw i32 %3, %2
+23 store i32 %add, ptr %result, align 4
+24 br label %for.inc
+*)
+
+
+definition mult_inc :: "llvm_instruction_block" where
+  "mult_inc = (
+    [],
+    [
+      load (lid ''4'') i32 (reg (lid ''i'')) (Some 4),
+      add (lid ''inc'') add_nsw i32 (reg (lid ''4'')) (val (vi32 1)),
+      store i32 (reg (lid ''inc'')) (reg (lid ''i'')) (Some 4)
+    ],
+    br_label (lid ''for.cond'')
+  )"
+
+
+(*
+26 for.inc:
+27 %4 = load i32, ptr %i, align 4
+28 %inc = add nsw i32 %4, 1
+29 store i32 %inc, ptr %i, align 4
+30 br label %for.cond
+*)
+
+
+definition mult_end :: "llvm_instruction_block" where
+  "mult_end = (
+    [],
+    [
+      load (lid ''5'') i32 (reg (lid ''result'')) (Some 4)
+    ],
+    ret (Some (i32, (reg (lid ''5''))))
+  )"
+
+definition mult_end_pre :: "state \<Rightarrow> state \<Rightarrow> bool" where
+  "mult_end_pre = (\<lambda>s s'. \<exists>aa a ba b ia i resa.
+    register_contains_value ((%''a.addr'')) (addr aa) s'
+  \<and> register_contains_value ((%''i''))      (addr ia) s'
+  \<and> register_contains_value ((%''b.addr'')) (addr ba) s'
+  \<and> register_contains_value ((%''result'')) (addr resa) s'
+
+  \<and> register_contains_value ((%''a'')) (vi32 a) s
+  \<and> register_contains_value ((%''b'')) (vi32 b) s
+  \<and> register_contains_value ((%''a'')) (vi32 a) s'
+  \<and> register_contains_value ((%''b'')) (vi32 b) s'
+
+  \<and> memory_\<alpha> s' = (memory_\<alpha> s)(
+      aa   := Some (mem_val (vi32 a)),
+      ba   := Some (mem_val (vi32 b)),
+      ia   := Some (mem_val (vi32 i)),
+      resa := Some (mem_val (vi32 (a*i)))
+    )
+  \<and> unique_addresses [aa, ba, ia, resa]
+  \<and> i = b
+  )"
+
+definition mult_post :: "postcondition" where
+  "mult_post = (\<lambda>s s' v. \<exists>a b i aa ba ia resa.
+    register_contains_value (lid ''a'') (vi32 a) s
+  \<and> register_contains_value (lid ''b'') (vi32 b) s
+  \<and> memory_\<alpha> s' = (memory_\<alpha> s)(
+      aa   := Some (mem_val (vi32 a)),
+      ba   := Some (mem_val (vi32 b)),
+      ia   := Some (mem_val (vi32 i)),
+      resa := Some (mem_val (vi32 (a*i)))
+    )
+  \<and> v = Some (vi32 (a * b))
+  )"
+
+(*
+32 for.end:
+33 %5 = load i32, ptr %result, align 4
+34 ret i32 %5
+*)
+
+
+definition mult_function :: llvm_function where
+  "mult_function = (func i32
+    [
+      (lid ''a'', i32),
+      (lid ''b'', i32)
+    ]
+    [
+      (lid ''entry'',    mult_entry),
+      (lid ''for.cond'', mult_cond),
+      (lid ''for.body'', mult_body),
+      (lid ''for.inc'',  mult_inc),
+      (lid ''for.end'',  mult_end)
+    ]
+  )"
+
+definition mult_program :: llvm_program where
+  "mult_program \<equiv> [
+    (gid ''mult'', mult_function)
+  ]"
+definition mult_annotations :: annotations where
+  "mult_annotations \<equiv>
+    [
+      (gid ''mult'',
+        (
+          mult_pre,
+          [
+            ((lid ''for.cond'', lid ''for.body''), mult_body_pre),
+            ((lid ''for.cond'', lid ''for.end'' ), mult_end_pre)
+          ],
+          mult_post
+        )
+      )
+    ]"
+
+
+lemma mult_floyd:
+  "verify_program
+    mult_program
+    mult_annotations"
+  including word_bundle
+  apply (vcg_verify_program prog: mult_program_def annot: mult_annotations_def)
+  apply (unfold_first_label func: mult_function_def)
+  apply (unfold_first_label func: mult_function_def)
+  
+  apply (intro allI impI conjI)
+
+  subgoal for s (* entry \<rightarrow> cond \<rightarrow> body *)
+    apply (vcg_floyd_cond prog: mult_program_def func: mult_function_def)
+    apply (unfold_precond pre: mult_pre_def)
+    apply (vcg_steps_execi block: mult_entry_def)
+    apply vcg_steps_execi
+    apply vcg_steps_execi
+    apply vcg_steps_execi
+    apply vcg_steps_execi
+    apply vcg_steps_execi
+    apply vcg_steps_execi
+    apply vcg_steps_execi
+    apply vcg_steps_execi
+    apply (vcg_steps_flowi_branch prog: mult_program_def annot: mult_annotations_def)
+    apply (vcg_step prog: mult_program_def func: mult_function_def)
+    apply (vcg_steps_execi block: mult_cond_def)
+    apply vcg_steps_execi
+    apply vcg_steps_execi
+    apply vcg_steps_execi
+    apply (vcg_steps_flowi_branch prog: mult_program_def annot: mult_annotations_def)
+    apply (vcg_annotation_holds prog: mult_program_def annot: mult_annotations_def pre: mult_body_pre_def)
+    apply (intro conjI)
+    subgoal
+      unfolding mult_pre_def
+      by blast
+    subgoal for a b aa ba ra ia s'
+      apply (rule exI[where x=aa])
+      apply (rule exI[where x=a])
+      apply (rule exI[where x=ba])
+      apply (rule exI[where x=b])
+      apply (rule exI[where x=ia])
+      apply (rule exI[where x=0])
+      apply (rule exI[where x=ra])
+      by (auto split: if_splits)
+    by blast
+
+  subgoal for init s (* body \<rightarrow> inc \<rightarrow> cond \<rightarrow> body or end *)
+    apply (vcg_floyd_cond prog: mult_program_def func: mult_function_def)
+    apply (unfold_precond prog: mult_program_def annot: mult_annotations_def pre: mult_body_pre_def mult_pre_def)
+    apply (vcg_steps_execi block: mult_body_def)
+    apply vcg_steps_execi
+    apply vcg_steps_execi apply (subst (asm) mult_pre_def) apply (clean_assms)
+    apply (intro wp_intro) apply simp apply simp subgoal apply (auto simp:  word_sless_alt word_sle_eq) sorry apply simp defer apply simp
+    apply vcg_steps_execi
+    apply vcg_steps_execi                                               
+    apply (vcg_steps_flowi_branch prog: mult_program_def annot: mult_annotations_def)
+    apply (vcg_step prog: mult_program_def func: mult_function_def)
+    apply (vcg_steps_execi block: mult_inc_def)
+    apply vcg_steps_execi
+    apply vcg_steps_execi
+    apply vcg_steps_execi
+    apply (vcg_steps_flowi_branch prog: mult_program_def annot: mult_annotations_def)
+    apply (vcg_step prog: mult_program_def func: mult_function_def)
+    apply (vcg_steps_execi block: mult_cond_def)
+    apply vcg_steps_execi
+    apply vcg_steps_execi
+    apply vcg_steps_execi 
+    subgoal for aa a ba b ia i ra s' (* cond \<rightarrow> body *)
+      apply (vcg_steps_flowi_branch prog: mult_program_def annot: mult_annotations_def)
+      apply (vcg_annotation_holds prog: mult_program_def annot: mult_annotations_def pre: mult_body_pre_def)
+      apply (intro conjI) unfolding mult_pre_def apply blast
+      
+      apply (rule exI[where x=aa])
+      apply (rule exI[where x=a])
+      apply (rule exI[where x=ba])
+      apply (rule exI[where x=b])
+      apply (rule exI[where x=ia])
+      apply (rule exI[where x="i+1"])
+      apply (rule exI[where x=ra]) 
+      by (auto simp: distrib_left)
+    subgoal for aa a ba b ia i ra s' (* cond \<rightarrow> end *)
+      apply (vcg_steps_flowi_branch prog: mult_program_def annot: mult_annotations_def)
+      apply (vcg_annotation_holds prog: mult_program_def annot: mult_annotations_def pre: mult_end_pre_def)
+      apply (intro conjI) unfolding mult_pre_def apply blast
+      apply (rule exI[where x=aa])
+      apply (rule exI[where x=a])
+      apply (rule exI[where x=ba])
+      apply (rule exI[where x=b])
+      apply (rule exI[where x=ia])
+      apply (rule exI[where x="i+1"])
+      apply (rule exI[where x=ra]) 
+      by auto
+    done
+
+  subgoal for init s (* end \<rightarrow> return *)
+    apply (vcg_floyd_cond prog: mult_program_def func: mult_function_def)
+    apply (unfold_precond prog: mult_program_def annot: mult_annotations_def pre: mult_end_pre_def)
+    apply (vcg_steps_execi block: mult_end_def)
+    apply vcg_steps_execi 
+    apply (vcg_steps_flowi_return prog: mult_program_def annot: mult_annotations_def)
+    apply (vcg_annotation_holds prog: mult_program_def annot: mult_annotations_def pre: mult_post_def)
+    apply (subst mult_program_def)
+    apply (intro conjI) defer unfolding mult_pre_def apply blast defer apply simp
+    subgoal for aa a ba b ia i resa s'
+      apply (rule exI[where x=a])
+      apply (rule exI[where x=b])
+      apply (rule exI[where x="b"])
+      apply (rule exI[where x=aa]) 
+      apply (rule exI[where x=ba]) 
+      apply (rule exI[where x=ia]) 
+      apply (rule exI[where x=resa])
+    by simp
+  done
+  done
+
+
+(*
+1 define dso_local noundef i32 @mult(int, int)(i32 noundef %a, i32 noundef %b) { llvm
+2 entry:
+3 %a.addr = alloca i32, align 4
+4 %b.addr = alloca i32, align 4
+5 %result = alloca i32, align 4
+6 %i = alloca i32, align 4
+7 store i32 %a, ptr %a.addr, align 4
+8 store i32 %b, ptr %b.addr, align 4
+9 store i32 0, ptr %result, align 4
+10 store i32 0, ptr %i, align 4
+11 br label %for.cond
+12
+13 for.cond:
+14 %0 = load i32, ptr %i, align 4
+15 %1 = load i32, ptr %b.addr, align 4
+16 %cmp = icmp slt i32 %0, %1
+17 br i1 %cmp, label %for.body, label %for.end
+18
+19 for.body:
+20 %2 = load i32, ptr %a.addr, align 4
+21 %3 = load i32, ptr %result, align 4
+22 %add = add nsw i32 %3, %2
+23 store i32 %add, ptr %result, align 4
+24 br label %for.inc
+25
+26 for.inc:
+27 %4 = load i32, ptr %i, align 4
+28 %inc = add nsw i32 %4, 1
+29 store i32 %inc, ptr %i, align 4
+30 br label %for.cond
+31
+32 for.end:
+33 %5 = load i32, ptr %result, align 4
+34 ret i32 %5
+35 }
+*)
+
+
+end
