VCG.thy
@@ -1,5 +1,5 @@
 theory VCG
-  imports "Steps" "HOL-Eisbach.Eisbach"
+  imports "Steps" "HOL-Eisbach.Eisbach" "Word_Lib/Word_32" "Word_Lib/Word_64"
 begin
 
 section "Useful Shorthands"
@@ -56,25 +56,27 @@ method repeat_minus_one methods m =
 method clean_registers = repeat_minus_one \<open>thin_tac "register_\<alpha> _ = _"\<close>
 method clean_memory = repeat_minus_one \<open>thin_tac "memory_\<alpha> _ = _"\<close>
 
-method clean_assms = ((elim exE conjE)+)?, (simp only: contract_updates)?; clean_registers?; clean_memory?; (simp only: triv_forall_equality)?
+method clean_assms = ((elim exE conjE allE)+)?, (simp only: contract_updates)?; clean_registers?; clean_memory?; (simp only: triv_forall_equality)?
+method clean_assms_non_destructive = ((elim exE conjE allE)+)?, (simp only: contract_updates)?; (simp only: triv_forall_equality)?
 
 method unfold_unique_addresses = simp only: registers_contain_unique_addresses.simps unique_addresses.simps unique_addresses_rec.simps unique_address.simps HOL.simp_thms(21), clean_assms
 
 subsection "Subgoal Solving Methods"
 
 method sub_instantiate_register_address = rule asm_rl[of "register_\<alpha> _ _ = Some (addr _)"], (fastforce | simp)?; fail
-method sub_memory_allocated = rule asm_rl[of "memory_\<alpha> _ _ \<noteq> None"], (fastforce | simp)?; fail
+method sub_memory_valid = rule asm_rl[of "valid_memory_address _ _"], (fastforce | simp)?; fail
 method sub_register_value = rule asm_rl[of "register_\<alpha> _ _ = Some _"], (fastforce | simp)?; fail
 method sub_memory_value = rule asm_rl[of "memory_\<alpha> _ _ = Some (mem_val _)"], (fastforce | simp split: if_splits)?; fail
-method sub_add_poison = (rule asm_rl[of "add_no_poison32 _ _ _"] | rule asm_rl[of "add_no_poison64 _ _ _"]), (fastforce | simp split: if_splits add: word_sless_alt word_sle_eq)?; fail
-method sub_icmp_same_signs = (rule asm_rl[of "if _ then same_signs32 _ _ else True"] | rule asm_rl[of "if _ then same_signs64 _ _ else True"]), (fastforce | simp split: if_splits add: word_sless_alt word_sle_eq)?; fail
+method sub_add_poison = (rule asm_rl[of "add_no_poison32 _ _ _"] | rule asm_rl[of "add_no_poison64 _ _ _"]), (simp split: if_splits add: word_sless_alt word_sle_eq signed.leD)?; fail
+method sub_icmp_same_signs = (rule asm_rl[of "if _ then same_signs32 _ _ else True"] | rule asm_rl[of "if _ then same_signs1 _ _ else True"] | rule asm_rl[of "if _ then same_signs64 _ _ else True"]), (fastforce | simp split: if_splits add: word_sless_alt word_sle_eq)?; fail
 method sub_map_of_some = rule asm_rl[of "map_of _ _ = Some _"], (fastforce | simp)?; fail
 method sub_distinct_first = rule asm_rl[of "distinct (map fst _)"], (fastforce | simp)?; fail
 method sub_some_refl = rule asm_rl[of "Some _ = Some _"], (rule refl)?; fail
+method sub_is_lid = rule asm_rl[of "is_lid _"], (fastforce | simp)?; fail
 
-method solve_subgoal = sub_instantiate_register_address | sub_memory_allocated | sub_register_value
+method solve_subgoal = sub_instantiate_register_address | sub_memory_valid | sub_register_value
                      | sub_memory_value | sub_add_poison | sub_icmp_same_signs | sub_map_of_some
-                     | sub_distinct_first | sub_some_refl
+                     | sub_distinct_first | sub_some_refl | sub_is_lid
 
 
 subsection "Instruction Methods"
@@ -82,11 +84,11 @@ subsection "Instruction Methods"
 method strat_instr methods m = rule wp_intro, m, clean_assms; (simp only: False_eq_False)?
 method strat_instr_dbg = (rule wp_intro, (solve_subgoal+)?); (rule asm_rl[of "wp _ _"], clean_assms)?; (simp only: False_eq_False)?
 
-method strat_alloca = rule asm_rl[of "wp (execute_alloca _ _) _"], strat_instr -
-method strat_store  = rule asm_rl[of "wp (execute_store _ _ _) _"], strat_instr \<open>sub_instantiate_register_address, sub_memory_allocated, sub_register_value\<close>
-method strat_load   = rule asm_rl[of "wp (execute_load _ _ _) _"], strat_instr \<open>sub_instantiate_register_address, sub_memory_value\<close>
-method strat_add    = rule asm_rl[of "wp (execute_add _ _ _ _ _) _"], strat_instr \<open>sub_register_value, sub_register_value, sub_add_poison\<close>
-method strat_icmp   = rule asm_rl[of "wp (execute_icmp _ _ _ _ _ _) _"], strat_instr \<open>sub_register_value, sub_register_value, sub_icmp_same_signs\<close>; simp only: compare_values_32.simps compare_values_64.simps
+method strat_alloca = rule asm_rl[of "wp (execute_alloca _ _) _"], strat_instr \<open>sub_is_lid\<close>
+method strat_store  = rule asm_rl[of "wp (execute_store _ _ _) _"], strat_instr \<open>sub_instantiate_register_address, sub_memory_valid, sub_register_value\<close>
+method strat_load   = rule asm_rl[of "wp (execute_load _ _ _) _"], strat_instr \<open>sub_instantiate_register_address, sub_memory_value, sub_is_lid\<close>
+method strat_add    = rule asm_rl[of "wp (execute_add _ _ _ _ _) _"], strat_instr \<open>sub_register_value, sub_register_value, sub_add_poison, sub_is_lid\<close>
+method strat_icmp   = rule asm_rl[of "wp (execute_icmp _ _ _ _ _ _) _"], strat_instr \<open>sub_register_value, sub_register_value, sub_icmp_same_signs, sub_is_lid\<close>; simp only: compare_values_32.simps compare_values_64.simps compare_values_1.simps
 
 method strat_alloca_dbg = rule asm_rl[of "wp (execute_alloca _ _) _"], strat_instr_dbg
 method strat_store_dbg  = rule asm_rl[of "wp (execute_store _ _ _) _"], strat_instr_dbg
@@ -96,14 +98,299 @@ method strat_icmp_dbg   = rule asm_rl[of "wp (execute_icmp _ _ _ _ _ _) _"], str
 
 method unfold_instr = rule asm_rl[of "wp (execute_instruction _ _) _"], rule wp_intro
 
-method instr_vcg_step = unfold_instr | strat_alloca | strat_store | strat_load | strat_add | strat_icmp
-method instr_vcg_step_dbg = unfold_instr | strat_alloca_dbg | strat_store_dbg | strat_load_dbg | strat_add_dbg | strat_icmp_dbg
+method vcg_instr = unfold_instr | strat_alloca | strat_store | strat_load | strat_add | strat_icmp
+method vcg_instr_dbg = unfold_instr | strat_alloca_dbg | strat_store_dbg | strat_load_dbg | strat_add_dbg | strat_icmp_dbg
 
 
 subsection "Phi Node Methods"
 
 method strat_phi = rule asm_rl[of "wp (execute_phi _ _ _) _"], strat_instr \<open>sub_distinct_first, sub_some_refl, sub_map_of_some, sub_register_value\<close>
 method strat_phi_dbg = rule asm_rl[of "wp (execute_phi _ _ _) _"], strat_instr_dbg
+
+
+
+
+
+
+
+
+
+
+
+
+
+
+
+
+
+
+
+method vcg_verify_function uses annot =
+  subst (3) annot,
+  simp del: split_paired_All,
+  intro conjI
+
+method vcg_verify_program uses prog annot =
+  simp,
+  subst prog,
+  simp,
+  (intro conjI)?; vcg_verify_function annot: annot
+
+method unfold_first_label uses func =
+  subst first_label_def,
+  subst func,
+  simp del: split_paired_All
+
+method vcg_step uses prog func =
+  rule wp_step_intro,
+  subst prog,
+  simp,
+  subst func,
+  simp
+
+method vcg_floyd_cond uses prog func =
+  subst floyd_cond_def,
+  rule wp_annotated_step_intro,
+  (vcg_step prog: prog func: func)
+
+
+method vcg_step_instr =
+  rule asm_rl[of "wp_rc_step_i _ _ (execi _ ([],_#_,_) _) _"],
+  intro wp_step_i_intros;
+  force?;
+  (thin_tac "\<not>is_call _" | thin_tac "is_call _")?,
+  (vcg_instr+)?
+method vcg_step_ter =
+  rule asm_rl[of "wp_rc_step_i _ _ (execi _ ([],[],_) _) _"],
+  intro wp_step_i_intros,
+  (simp; fail)?;
+  (thin_tac "\<not>is_call _" | thin_tac "is_call _")?
+
+method vcg_steps_execi uses block =
+  rule asm_rl[of "wp_rc_steps_i _ _ (execi _ _ _) _"],
+  rule wp_rc_steps_i_intro;
+  (simp; fail)?;
+  (thin_tac "\<not>(_ \<nexists>\<rightarrow>\<^sub>i)" | thin_tac "_ \<nexists>\<rightarrow>\<^sub>i")?,
+  (subst block)?,
+  (vcg_step_instr | vcg_step_ter)
+
+method vcg_steps_flowi_branch uses block pre prog annot =
+  rule asm_rl[of "wp_rc_steps_i _ _ (flowi _ (branch_label _)) _"],
+  rule wp_rc_steps_i_intro;
+  (simp; fail)?;
+  (thin_tac "\<not>(_ \<nexists>\<rightarrow>\<^sub>i)" | thin_tac "_ \<nexists>\<rightarrow>\<^sub>i")?,
+  simp (no_asm),
+  rule wp_steps_until_intro;
+  ((subst (asm) has_annotation_def, subst (asm) prog, subst (asm) annot, simp); fail)?,
+  (thin_tac "has_annotation _ _ _" | thin_tac "\<not>has_annotation _ _ _")?
+
+method vcg_steps_flowi_return uses block pre prog annot =
+  rule asm_rl[of "wp_rc_steps_i _ _ (flowi _ (return_value _)) _"],
+  rule wp_rc_steps_i_intro;
+  (simp; fail)?;
+  (thin_tac "\<not>(_ \<nexists>\<rightarrow>\<^sub>i)" | thin_tac "_ \<nexists>\<rightarrow>\<^sub>i")?,
+  simp (no_asm),
+  rule wp_steps_until_intro;
+  ((subst (asm) has_annotation_def, subst (asm) prog, subst (asm) annot, simp); fail)?,
+  (thin_tac "has_annotation _ _ _" | thin_tac "\<not>has_annotation _ _ _")?
+
+method vcg_steps uses block pre =
+  rule wp_rc_steps_i_intro;
+  (simp; fail)?;
+  (thin_tac "\<not>(_ \<nexists>\<rightarrow>\<^sub>i)" | thin_tac "_ \<nexists>\<rightarrow>\<^sub>i")?,
+  (subst block)?,
+  (subst (asm) pre)?
+
+method vcg_annotation_holds uses prog annot pre =
+  subst annotation_holds_def,
+  subst prog,
+  subst annot,
+  (simp (no_asm) del: split_paired_All)?,
+  unfold pre,
+  (simp (no_asm) del: split_paired_All)?
+
+
+method unfold_precond uses pre annot prog =
+  (subst (asm) annotation_holds_def,
+  subst (asm) annot,
+  subst (asm) prog)?,
+  (simp (no_asm_use) del: split_paired_All)?,
+  subst (asm) pre,
+  clean_assms
+
+
+
+
+
+
+
+
+
+
+
+
+
+
+
+
+
+
+
+
+
+section "Word Lemma Bundle"
+
+bundle word_bundle
+begin
+
+lemma lt_imp_le: "(i::word32) <s 2 ^ 31 - 1 \<Longrightarrow> i \<le>s 2 ^ 31 - 2"
+  by (simp add: word_sle_eq word_sless_alt)
+
+
+lemma le_imp_lt: "i \<le>s 2 ^ 31 - 2 \<Longrightarrow> (i::word32) <s 2 ^ 31 - 1"
+  by (simp add: word_sle_eq word_sless_alt)
+
+lemma lt_inc_nlt_imp_eq[simp]: "(i::word32) <s (b::word32) \<Longrightarrow> \<not> i+1 <s b \<Longrightarrow> i+1 = b"
+  apply (simp add: word_sle_eq word_sless_alt)
+  by (smt (verit, ccfv_threshold) diff_add_cancel signed_arith_ineq_checks_to_eq_word32(1,2) signed_minus_1
+      signed_take_bit_int_eq_self signed_take_bit_int_greater_eq_minus_exp sint_word_ariths(1,8) word_sint.Rep_eqD)
+
+lemma lt_inc_nlt_mult_eq[simp]: "(i::word32) <s (b::word32) \<Longrightarrow> \<not> i+1 <s b \<Longrightarrow> a*i+a = a*b"
+  by (metis (no_types, lifting) distrib_left lt_inc_nlt_imp_eq mult_numeral_1_right numeral_One)
+
+lemma i_no_overflow_impl_positive[simp]: "0 \<le>s i \<Longrightarrow> (i::word32) <s 2^31 - 1 \<Longrightarrow> 0 \<le>s (i+1)"
+  by (smt (verit, del_insts) add_diff_eq diff_add_cancel diff_numeral_special(10) of_int_eq_id signed_minus_1
+      signed_take_bit_int_eq_self signed_take_bit_int_eq_self_iff signed_take_bit_int_greater_eq_minus_exp sint_word_ariths(1,2,8)
+      word_sle_eq word_sless_alt)
+
+lemma i_incr_no_overflow_impl_not_negative[simp]: "0 \<le>s (i::word32) \<Longrightarrow> (i::word32) <s 2^31 - 1 \<Longrightarrow> \<not> i + 1 <s 0"
+  by (smt (verit, best) i_no_overflow_impl_positive word_sle_eq word_sless_alt)
+
+lemma i_bounds_no_overflow_neg[simp]: "- (2 ^ 31) \<le> sint (a::word32) * sint (b::word32) \<Longrightarrow>
+    sint a * sint b \<le> 2 ^ 31 - 1 \<Longrightarrow>
+    0 \<le>s (i::word32) \<Longrightarrow>
+    i <s b \<Longrightarrow>
+    b \<le>s 2 ^ 31 - 1 \<Longrightarrow>
+    i <s 2 ^ 31 - 1 \<Longrightarrow>
+    a <s 0 \<Longrightarrow> a * i <s 0 \<Longrightarrow> \<not> 0 \<le>s a * i + a"
+proof -
+  assume bounds: "- (2^31) \<le> sint a * sint b" "sint a * sint b \<le> 2^31 - 1"
+  assume hi: "0 \<le>s i" "i <s b" "b \<le>s 2^31 - 1" "i <s 2^31 - 1"
+  assume neg: "a <s 0" "a * i <s 0"
+  have sa: "sint a < 0"
+    using neg(1) 
+    by (simp add: word_sless_alt)
+  have si: "0 \<le> sint i"
+    using hi(1)
+    by (simp add: word_sless_alt word_sle_eq)
+  have si_lt: "sint i < 2^31 - 1"
+    using hi(4) by (simp add: word_sless_alt word_sle_eq)
+  have sb_lt: "sint b \<le> 2^31 - 1"
+    using hi(3) by (simp add: word_sless_alt word_sle_eq)
+  have sai_neg: "sint (a * i) < 0"
+    using neg(2) by (simp add: word_sless_alt word_sle_eq)
+  have no_ovf_ai: "sint (a * i) = sint a * sint i"
+    using sai_neg sa si 
+    apply(auto intro: signed_arith_sint simp: sint_word_ariths word_sless_alt word_sle_eq)
+    by (smt (verit, del_insts) bounds(1) hi(2) mult_eq_0_iff mult_less_cancel_left_disj signed_take_bit_int_eq_self
+        word_sless_alt)
+  have no_ovf_sum: "sint (a * i + a) = sint (a * i) + sint a"
+    proof -
+      have lo: "-(2^31) \<le> sint (a * i) + sint a"
+      proof -
+        have si_lt_b: "sint i < sint b"
+          using hi(2) by (simp add: word_sless_alt)
+        have sb_bounds: "-(2^31) \<le> sint b"
+          using si si_lt_b by auto
+        have key: "sint a * sint b \<le> sint a * (sint i + 1)"
+          using sa si_lt_b
+          by (simp add: mult_le_cancel_left_neg)
+        show ?thesis
+          using no_ovf_ai key bounds(1) right_diff_distrib' mult_cancel_left2
+          by (smt (verit) )
+      qed
+      have hi': "sint (a * i) + sint a \<le> 2^31 - 1"
+        using sai_neg sa
+        by simp
+      then show ?thesis
+        using lo hi' no_ovf_ai
+        by (simp add: sint_word_ariths signed_take_bit_int_eq_self)
+    qed
+  show "\<not> 0 \<le>s a * i + a"
+    unfolding word_sle_def
+    using no_ovf_sum sai_neg sa
+    by (smt (verit) neg(1) word_sle_def word_sle_eq word_sless_alt)
+qed
+
+lemma i_bounds_no_overflow_pos[simp]: "- (2 ^ 31) \<le> sint (a::word32) * sint (b::word32) \<Longrightarrow>
+    sint a * sint b \<le> 2 ^ 31 - 1 \<Longrightarrow>
+    0 <s b \<Longrightarrow>
+    0 \<le>s (i::word32) \<Longrightarrow>
+    i <s b \<Longrightarrow>
+    b \<le>s 2 ^ 31 - 1 \<Longrightarrow>
+    i <s 2 ^ 31 - 1 \<Longrightarrow>
+    0 \<le>s a \<Longrightarrow> 0 \<le>s a * i \<Longrightarrow> \<not> a * i + a <s 0"
+proof -
+  assume bounds: "- (2^31) \<le> sint a * sint b" "sint a * sint b \<le> 2^31 - 1"
+  assume hi: "0 \<le>s i" "i <s b" "b \<le>s 2^31 - 1" "i <s 2^31 - 1"
+  assume pos: "0 \<le>s a" "0 \<le>s a * i"
+  have sa: "sint a \<ge> 0"
+    using pos(1)
+    by (simp add: word_sle_eq)
+  have si: "0 \<le> sint i"
+    using hi(1)
+    by (simp add: word_sless_alt word_sle_eq)
+  have si_lt: "sint i < 2^31 - 1"
+    using hi(4) by (simp add: word_sless_alt word_sle_eq)
+  have sb_lt: "sint b \<le> 2^31 - 1"
+    using hi(3) by (simp add: word_sless_alt word_sle_eq)
+  have sai_neg: "sint (a * i) \<ge> 0"
+    using pos(2) by (simp add: word_sless_alt word_sle_eq)
+  have no_ovf_ai: "sint (a * i) = sint a * sint i"
+    using sai_neg sa si 
+    apply(auto intro: signed_arith_sint simp: sint_word_ariths word_sless_alt word_sle_eq)
+    by (smt (verit, best) bounds(2) hi(2) mult_less_cancel_left_disj signed_take_bit_int_eq_self word_sless_alt
+        zero_le_mult_iff)
+  have no_ovf_sum: "sint (a * i + a) = sint (a * i) + sint a"
+    proof -
+      have lo: "-(2^31) \<le> sint (a * i) + sint a"
+        using sa sai_neg by force
+      have hi': "sint (a * i) + sint a \<le> 2^31 - 1"
+      proof -
+        have si_lt_b: "sint i < sint b"
+          using hi(2) by (simp add: word_sless_alt)
+        have sb_bounds: "-(2^31) \<le> sint b"
+          using si si_lt_b by auto
+        have key: "sint a * sint b \<ge> sint a * (sint i + 1)"
+          using sa si_lt_b
+          by (smt (verit, best) mult_less_cancel_left_disj)
+        show ?thesis
+          using no_ovf_ai key bounds(2) right_diff_distrib' mult_cancel_left2
+          by (smt (verit, best))
+      qed
+      then show ?thesis
+        using lo hi' no_ovf_ai
+        by (simp add: sint_word_ariths signed_take_bit_int_eq_self)
+    qed
+  show ?thesis
+    unfolding word_sle_def
+    using no_ovf_sum sai_neg sa 
+    by (smt (verit) pos(1) word_sle_def word_sle_eq word_sless_alt)
+qed
+
+lemma bounded_inc_no_overflow[simp]: "0 \<le>s i \<Longrightarrow> (b::word32) \<le>s 2^31-1 \<Longrightarrow> (i::word32) <s b \<Longrightarrow> 0 <s i+1"
+  using sint_word_ariths word_sle_eq word_sless_alt add_diff_cancel_right' i_incr_no_overflow_impl_not_negative signed_0 signed_minus_1
+  by (smt (verit, del_insts))
+lemma pos_not_neg[simp]: "0 <s (i::word32)+1 \<Longrightarrow> \<not> i + 1 <s 0" by simp
+
+end
+
+
+
+
+
+
+
 
 method unfold_wp_instrs_phi = rule asm_rl[of "wp_instrs _ (execi _ (_#_,_,_) _) _"], rule wp_instrs_intro
 
